pushing toString functions to HOL

Examples/Code_Interface.thy
@@ -32,9 +32,10 @@ definition upper_closure :: "common_primitive rule list \<Rightarrow> common_pri
 definition lower_closure :: "common_primitive rule list \<Rightarrow> common_primitive rule list" where
   "lower_closure rs == transform_optimize_dnf_strict (transform_normalize_primitives (transform_optimize_dnf_strict (optimize_matches_a lower_closure_matchexpr rs)))"
 
+(*
 definition port_to_nat :: "16 word \<Rightarrow> nat" where
   "port_to_nat p = unat p"
-
+*)
 
 
 
@@ -44,5 +45,46 @@ lemma "bitmask_to_strange_inverse_cisco_mask 16 = (0, 0, 255, 255)" by eval
 lemma "bitmask_to_strange_inverse_cisco_mask 24 = (0, 0, 0, 255)" by eval
 lemma "bitmask_to_strange_inverse_cisco_mask 8 = (0, 255, 255, 255)" by eval
 lemma "bitmask_to_strange_inverse_cisco_mask 32 = (0, 0, 0, 0)" by eval
+
+
+subsection{*toString functions*}
+(*http://stackoverflow.com/questions/23864965/string-of-nat-in-isabelle*)
+fun string_of_nat :: "nat \<Rightarrow> string" where
+  "string_of_nat n = (if n < 10 then [char_of_nat (48 + n)] else 
+     string_of_nat (n div 10) @ [char_of_nat (48 + (n mod 10))])"
+definition string_of_int :: "int \<Rightarrow> string" where
+  "string_of_int i = (if i < 0 then ''-'' @ string_of_nat (nat (- i)) else 
+     string_of_nat (nat i))"
+
+definition ipv4_cidr_toString :: "(ipv4addr \<times> nat) \<Rightarrow> string" where
+  "ipv4_cidr_toString ip_n = (case ip_n of (base, n) \<Rightarrow> 
+      (case dotdecimal_of_ipv4addr base of (a,b,c,d) \<Rightarrow> string_of_nat a @''.''@ string_of_nat b @''.''@ string_of_nat c @''.''@ string_of_nat d
+          @''/''@ string_of_nat n))"
+lemma "ipv4_cidr_toString (ipv4addr_of_dotdecimal (192,168,0,1), 22) = ''192.168.0.1/22''" by eval
+
+fun protocol_toString :: "protocol \<Rightarrow> string" where
+  "protocol_toString (ProtoAny) = ''all''" |
+  "protocol_toString (Proto TCP) = ''tcp''" |
+  "protocol_toString (Proto UDP) = ''udp''" |
+  "protocol_toString (Proto ICMP) = ''icmp''"
+
+fun simple_action_toString :: "simple_action \<Rightarrow> string" where
+  "simple_action_toString Accept = ''ACCEPT''" |
+  "simple_action_toString Drop = ''DROP''"
+
+definition port_toString :: "16 word \<Rightarrow> string" where
+  "port_toString p \<equiv> string_of_nat (unat p)"
+
+definition iface_toString :: "string \<Rightarrow> iface \<Rightarrow> string" where
+  "iface_toString descr iface = (if iface = IfaceAny then '''' else
+      (case iface of (Iface name) \<Rightarrow> descr@name))"
+lemma "iface_toString ''src: '' (Iface ''+'') = ''''" by eval
+lemma "iface_toString ''src: '' (Iface ''eth0'') = ''src: eth0''" by eval
+
+fun ports_toString :: "string \<Rightarrow> (16 word \<times> 16 word) \<Rightarrow> string" where
+  "ports_toString descr (s,e) = (if s = 0 \<and> e = max_word then '''' else descr@''(''@port_toString s@'',''@port_toString e@'')'')"
+lemma "ports_toString ''src: '' (0,65535) = ''''" by eval
+lemma "ports_toString ''src: '' (1024,2048) = ''src: (1024,2048)''" by eval
+
 
 end
